James C - better program states for assembly

AssemblyLanguage.thy
@@ -11,24 +11,25 @@ datatype assembly =
 
 type_synonym program = "symbol \<leadsto> assembly list"
 
-type_synonym assembly_state = "memory \<times> int \<times> int \<times> assembly list" (* M, A, D, PC *)
+type_synonym assembly_state = "memory \<times> int option \<times> int \<times> assembly list" (* M, A, D, PC *)
 
 fun eval_assembly :: "program \<Rightarrow> assembly_state \<Rightarrow> assembly_state option" where
   "eval_assembly \<Pi> (\<sigma>, a, d, []) = None"
-| "eval_assembly \<Pi> (\<sigma>, a, d, AAssm x # \<pi>) = Some (\<sigma>, x, d, \<pi>)"
-| "eval_assembly \<Pi> (\<sigma>, a, d, CAssm dst cmp # \<pi>) = (
+| "eval_assembly \<Pi> (\<sigma>, a, d, AAssm x # \<pi>) = Some (\<sigma>, Some x, d, \<pi>)"
+| "eval_assembly \<Pi> (\<sigma>, Some a, d, CAssm dst cmp # \<pi>) = (
     let n = compute cmp (\<sigma> a) a d
     in Some (
       if M \<in> dst then \<sigma>(a := n) else \<sigma>, 
-      if A \<in> dst then n else a, 
+      Some (if A \<in> dst then n else a), 
       if D \<in> dst then n else d, 
       \<pi>))"
+| "eval_assembly \<Pi> (\<sigma>, None, d, CAssm dst cmp # \<pi>) = None"
 | "eval_assembly \<Pi> (\<sigma>, a, d, JAssm jmp s # \<pi>) = (
     if should_jump d jmp
     then case lookup \<Pi> s of 
-        Some \<pi>' \<Rightarrow> Some (\<sigma>, a, d, \<pi>')
+        Some \<pi>' \<Rightarrow> Some (\<sigma>, None, d, \<pi>')
       | None \<Rightarrow> None
-    else Some (\<sigma>, a, d, \<pi>))"
+    else Some (\<sigma>, None, d, \<pi>))"
 
 (* conversion *)
 
@@ -62,12 +63,21 @@ definition get_pc :: "program \<Rightarrow> assembly list \<Rightarrow> nat set"
   "get_pc \<Pi> \<pi> = { the (build_symbol_table \<Pi> s) + length \<pi>' | s \<pi>'. lookup \<Pi> s = Some (\<pi>' @ \<pi>) }"
 
 fun state_convert :: "program \<Rightarrow> assembly_state \<Rightarrow> machine_state set" where
-  "state_convert \<Pi> (\<sigma>, a, d, \<pi>) = (\<lambda>pc. (\<sigma>, a, d, pc)) ` get_pc \<Pi> \<pi>"
+  "state_convert \<Pi> (\<sigma>, Some a, d, \<pi>) = {(\<sigma>, a, d, pc) | pc. pc \<in> get_pc \<Pi> \<pi>}"
+| "state_convert \<Pi> (\<sigma>, None, d, \<pi>) = {(\<sigma>, a, d, pc) | a pc. pc \<in> get_pc \<Pi> \<pi>}"
 
 (* conversion correctness *)
 
 lemma [simp]: "lookup \<Pi> s = Some \<pi> \<Longrightarrow> \<exists>n. build_symbol_table \<Pi> s = Some n"
   by (induction \<Pi> s rule: lookup.induct) auto
+
+lemma [simp]: "lookup \<Pi> s = Some \<pi> \<Longrightarrow> nat (get_block_addr (build_symbol_table \<Pi>) s) \<in> get_pc \<Pi> \<pi>" 
+  proof (induction \<Pi> s rule: lookup.induct)
+  case 1
+    thus ?case by simp
+  next case 2
+    thus ?case by simp
+  qed
 
 lemma convert_expands [simp]: "length \<pi> \<le> get_converted_length \<pi>"
   by (induction \<pi> rule: get_converted_length.induct) simp_all
@@ -97,16 +107,26 @@ lemma [simp]: "lookup \<Pi> s = Some (\<pi> @ \<pi>') \<Longrightarrow> \<pi>' \
       qed
   qed
 
-lemma [simp]: "pc \<in> get_pc \<Pi> (a # \<pi>) \<Longrightarrow>
-    program_convert \<Pi> ! pc = hd (instruction_conv (build_symbol_table \<Pi>) a)"
-  by (auto simp add: get_pc_def program_convert_def)
-
-lemma [simp]: "pc \<in> get_pc \<Pi> (a # \<pi>) \<Longrightarrow> length (instruction_conv (build_symbol_table \<Pi>) a) = 1 \<Longrightarrow>
-    program_convert \<Pi> ! (Suc pc) = hd (tl (instruction_conv (build_symbol_table \<Pi>) a))"
-  by (auto simp add: get_pc_def program_convert_def)
-
 lemma [simp]: "pc \<in> get_pc \<Pi> (a # \<pi>) \<Longrightarrow> pc < length (program_convert \<Pi>)"
   by (auto simp add: get_pc_def)
+
+lemma [simp]: "pc \<in> get_pc \<Pi> (JAssm jmp s # \<pi>) \<Longrightarrow> Suc pc < length (program_convert \<Pi>)"
+  by (auto simp add: get_pc_def)
+
+lemma lookup_convert: "pc \<in> get_pc \<Pi> (a # \<pi>) \<Longrightarrow> 
+  i < length (instruction_conv (build_symbol_table \<Pi>) a) \<Longrightarrow>
+    program_convert \<Pi> ! (pc + i) = instruction_conv (build_symbol_table \<Pi>) a ! i"
+  proof -
+    assume "i < length (instruction_conv (build_symbol_table \<Pi>) a)"
+    assume "pc \<in> get_pc \<Pi> (a # \<pi>)" 
+    then obtain s \<pi>' where P :"pc = the (build_symbol_table \<Pi> s) + length \<pi>' \<and> 
+      lookup \<Pi> s = Some (\<pi>' @ a # \<pi>)" by (auto simp add: get_pc_def)
+
+
+    have "concat (map (instruction_conv (build_symbol_table \<Pi>)) (get_assembly \<Pi>)) ! (the (build_symbol_table \<Pi> s) + length \<pi>' + i) = 
+      instruction_conv (build_symbol_table \<Pi>) a ! i" by simp
+    with P show ?thesis by (simp add: program_convert_def)
+  qed
 
 lemma [simp]: "pc \<in> get_pc \<Pi> (a # \<pi>) \<Longrightarrow> Suc pc \<in> get_pc \<Pi> \<pi>"
   proof -
@@ -115,31 +135,74 @@ lemma [simp]: "pc \<in> get_pc \<Pi> (a # \<pi>) \<Longrightarrow> Suc pc \<in> 
       lookup \<Pi> s = Some (\<pi>' @ a # \<pi>)" by (auto simp add: get_pc_def)
     hence "the (build_symbol_table \<Pi> s) + length (\<pi>' @ [a]) \<in> 
       { the (build_symbol_table \<Pi> s) + length \<pi>' | s \<pi>'. lookup \<Pi> s = Some (\<pi>' @ \<pi>) }" by fastforce
-    with P show "Suc pc \<in> get_pc \<Pi> \<pi>" by (simp add: get_pc_def)
+    with P show ?thesis by (simp add: get_pc_def)
   qed
 
+lemma [simp]: "pc \<in> get_pc \<Pi> (JAssm jmp s # \<pi>) \<Longrightarrow> Suc (Suc pc) \<in> get_pc \<Pi> \<pi>"
+  proof -
+    assume "pc \<in> get_pc \<Pi> (JAssm jmp s # \<pi>)"
+    have "Suc (Suc pc) \<in> get_pc \<Pi> \<pi>" by simp
+    thus ?thesis by simp
+  qed
+
+lemma [simp]: "\<Sigma> \<in> state_convert \<Pi> (\<sigma>, a, d, \<pi>) \<Longrightarrow> \<exists>aa pc. \<Sigma> = (\<sigma>, aa, d, pc) \<and> pc \<in> get_pc \<Pi> \<pi>"
+  by (cases a) auto
+
 lemma eval_assembly_conv [simp]: "eval_assembly \<Pi> \<Sigma> = Some \<Sigma>\<^sub>1 \<Longrightarrow> \<Sigma>' \<in> state_convert \<Pi> \<Sigma> \<Longrightarrow>
-    \<exists>\<Sigma>\<^sub>1'. \<Sigma>\<^sub>1' \<in> state_convert \<Pi> \<Sigma>\<^sub>1 \<and> eval (program_convert \<Pi>) \<Sigma>' = Some \<Sigma>\<^sub>1'"
+    \<exists>\<Sigma>\<^sub>1'. \<Sigma>\<^sub>1' \<in> state_convert \<Pi> \<Sigma>\<^sub>1 \<and> iterate (eval (program_convert \<Pi>)) \<Sigma>' \<Sigma>\<^sub>1'"
   proof (induction \<Pi> \<Sigma> rule: eval_assembly.induct)
   case 1
     thus ?case by simp
-  next case 2
-    thus ?case by auto
+  next case (2 \<Pi> \<sigma> a d x \<pi>)
+    from 2 have S: "\<Sigma>\<^sub>1 = (\<sigma>, Some x, d, \<pi>)" by simp
+    from 2 obtain pc aa where P: "\<Sigma>' = (\<sigma>, aa, d, pc) \<and> pc \<in> get_pc \<Pi> (AAssm x # \<pi>)" by fastforce
+    hence X: "(\<sigma>, x, d, Suc pc) \<in> state_convert \<Pi> (\<sigma>, Some x, d, \<pi>)" by auto
+    from P lookup_convert have "eval (program_convert \<Pi>) (\<sigma>, aa, d, pc) = Some (\<sigma>, x, d, Suc pc)" 
+      by fastforce
+    with X S P show ?case by fast
   next case (3 \<Pi> \<sigma> a d dst cmp \<pi>)
     let ?n = "compute cmp (\<sigma> a) a d"
-    from 3 have S: " \<Sigma>\<^sub>1 = (
-      if M \<in> dst then \<sigma>(a := ?n) else \<sigma>, 
-      if A \<in> dst then ?n else a, 
-      if D \<in> dst then ?n else d, 
-      \<pi>)" by (simp add: Let_def)
-    from 3 have "\<Sigma>' \<in> state_convert \<Pi> (\<sigma>, a, d, CAssm dst cmp # \<pi>)" by simp
-
-
-    have "\<Sigma>\<^sub>1' \<in> (\<lambda>pc. (if M \<in> dst then \<sigma>(a := ?n) else \<sigma>, if A \<in> dst then ?n else a, if D \<in> dst then ?n else d, pc)) ` get_pc \<Pi> \<pi> \<and> 
-      eval (program_convert \<Pi>) \<Sigma>' = Some \<Sigma>\<^sub>1'" by simp
-    with S show ?case by fastforce
+    let ?\<sigma> = "if M \<in> dst then \<sigma>(a := ?n) else \<sigma>"
+    let ?a = "if A \<in> dst then ?n else a"
+    let ?d = "if D \<in> dst then ?n else d"
+    from 3 have S: "\<Sigma>\<^sub>1 = (?\<sigma>, Some ?a, ?d, \<pi>)" by (simp add: Let_def)
+    from 3 obtain pc where P: "\<Sigma>' = (\<sigma>, a, d, pc) \<and> pc \<in> get_pc \<Pi> (CAssm dst cmp # \<pi>)" by fastforce
+    hence X: "(?\<sigma>, ?a, ?d, Suc pc) \<in> state_convert \<Pi> (?\<sigma>, Some ?a, ?d, \<pi>)" by auto
+    have "eval_instruction (CInstr dst cmp {}) (\<sigma>, a, d, pc) = (?\<sigma>, ?a, ?d, Suc pc)" 
+      by (simp add: Let_def)
+    with P lookup_convert have "eval (program_convert \<Pi>) (\<sigma>, a, d, pc) = Some (?\<sigma>, ?a, ?d, Suc pc)" 
+      by fastforce
+    with X S P show ?case by fast
   next case 4
     thus ?case by simp
+  next case (5 \<Pi> \<sigma> a d jmp s \<pi>)
+    then obtain pc aa where P: "\<Sigma>' = (\<sigma>, aa, d, pc) \<and> pc \<in> get_pc \<Pi> (JAssm jmp s # \<pi>)" by fastforce
+    let ?s = "get_block_addr (build_symbol_table \<Pi>) s"
+    from P lookup_convert have first_step: "eval (program_convert \<Pi>) (\<sigma>, aa, d, pc) = 
+      Some (\<sigma>, ?s, d, Suc pc)" by fastforce
+    show ?case
+      proof (cases "should_jump d jmp")
+      case True
+        thus ?thesis
+          proof (cases "lookup \<Pi> s")
+          case (Some \<pi>')
+            with 5 True have S: "\<Sigma>\<^sub>1 = (\<sigma>, None, d, \<pi>')" by simp
+            from Some have X: "(\<sigma>, ?s, d, nat ?s) \<in> state_convert \<Pi> (\<sigma>, None, d, \<pi>')" by simp
+            from P lookup_convert True have "eval (program_convert \<Pi>) (\<sigma>, ?s, d, Suc pc) = 
+              Some (\<sigma>, ?s, d, nat ?s)" by fastforce
+            with first_step X P S show ?thesis by fast
+          next case None
+            with 5 True show ?thesis by simp
+          qed
+      next case False
+        from 5 False have S: "\<Sigma>\<^sub>1 = (\<sigma>, None, d, \<pi>)" by auto
+        from P have X: "(\<sigma>, ?s, d, Suc (Suc pc)) \<in> state_convert \<Pi> (\<sigma>, None, d, \<pi>)" by auto
+        from False have "eval_instruction (CInstr {} (Reg D) jmp) (\<sigma>, ?s, d, Suc pc) = 
+          (\<sigma>, ?s, d, Suc (Suc pc))" by auto
+        with P lookup_convert have "eval (program_convert \<Pi>) (\<sigma>, ?s, d, Suc pc) =
+          Some (\<sigma>, ?s, d, Suc (Suc pc))" by fastforce
+        with first_step X P S show ?thesis by fast
+      qed
   qed
 
 theorem [simp]: "iterate (eval_assembly \<Pi>) \<Sigma> \<Sigma>\<^sub>1 \<Longrightarrow> \<Sigma>' \<in> state_convert \<Pi> \<Sigma> \<Longrightarrow> 
@@ -151,7 +214,7 @@ theorem [simp]: "iterate (eval_assembly \<Pi>) \<Sigma> \<Sigma>\<^sub>1 \<Longr
     then obtain \<Sigma>\<^sub>1' where S: "\<Sigma>\<^sub>1' \<in> state_convert \<Pi> \<Sigma>\<^sub>1 \<and> 
       iterate (eval (program_convert \<Pi>)) \<Sigma>' \<Sigma>\<^sub>1'" by blast
     with iter_step eval_assembly_conv obtain \<Sigma>\<^sub>2' where
-      "\<Sigma>\<^sub>2' \<in> state_convert \<Pi> \<Sigma>\<^sub>2 \<and> eval (program_convert \<Pi>) \<Sigma>\<^sub>1' = Some \<Sigma>\<^sub>2'" by blast
+      "\<Sigma>\<^sub>2' \<in> state_convert \<Pi> \<Sigma>\<^sub>2 \<and> iterate (eval (program_convert \<Pi>)) \<Sigma>\<^sub>1' \<Sigma>\<^sub>2'" by blast
     with S have "\<Sigma>\<^sub>2' \<in> state_convert \<Pi> \<Sigma>\<^sub>2 \<and> iterate (eval (program_convert \<Pi>)) \<Sigma>' \<Sigma>\<^sub>2'" 
       by fastforce
     thus ?case by blast
